ipassmt debug algorithm

Examples/Code_haskell.thy
@@ -71,9 +71,6 @@ definition "example_TUM_i8_spoofing_ipassmt =
     (ipv4addr_of_dotdecimal (185,86,232,0), 22)
     ]) (*transfer net*)]"
 
-definition map_of_ipassmt :: "(iface \<times> (32 word \<times> nat) list) list \<Rightarrow> iface \<rightharpoonup> (32 word \<times> nat) list" where
-  "map_of_ipassmt ipassmt = map_of ipassmt"
-
 
 fun ipassmt_iprange_translate :: "ipt_ipv4range list negation_type \<Rightarrow> (32 word \<times> nat) list" where
   "ipassmt_iprange_translate (Pos ips) = concat (map ipt_ipv4range_to_cidr ips)" |
@@ -102,7 +99,8 @@ export_code Rule
   to_simple_firewall
   to_simple_firewall_without_interfaces
   sanity_wf_ruleset
-  (*spoofing:*) example_TUM_i8_spoofing_ipassmt no_spoofing_iface ipassmt_sanity_defined map_of_ipassmt to_ipassmt
+  (*spoofing:*) example_TUM_i8_spoofing_ipassmt
+  no_spoofing_iface ipassmt_sanity_defined map_of_ipassmt to_ipassmt ipassmt_sanity_nowildcards
   Pos Neg
   in Haskell module_name "Network.IPTables.Generated" file "generated_code/"
 
